src/tosmt/z3.fs
@@ -45,6 +45,10 @@ let status_to_string = function
     | UNKNOWN -> "unknown"
     | TIMEOUT -> "timeout"
 
+let z3proc = 
+    let cond (s:string) = Util.trim_string s = "Done!" in
+    Util.start_process "z3.exe" ini_params cond 
+
 let doZ3Exe (input:string) = 
   let parse (z3out:string) = 
     let lines = String.split ['\n'] z3out |> List.map Util.trim_string in
@@ -60,31 +64,34 @@ let doZ3Exe (input:string) =
       | _::tl -> result tl 
       | _ -> failwith <| format1 "Got output lines: %s\n" (String.concat "\n" (List.map (fun (l:string) -> format1 "<%s>" (Util.trim_string l)) lines)) in
       result lines in
-  let cond (s:string) = Util.trim_string s = "Done!" in
-  let z3proc = Util.start_process "z3.exe" ini_params cond in
   let stdout = Util.ask_process z3proc input in    
-  let _ = Util.kill_all () in //process z3proc in
   parse (Util.trim_string stdout) 
 
-let qfile = 
-    let ctr = Util.mk_ref 0 in
-    (fun () -> 
-        incr ctr;
-        let fname = format1 "query-%s.smt2" (string_of_int !ctr) in
-        Util.print_string (Util.format1 "Writing to file %s\n" fname);
-        fname)
+let qfh : ref<option<Util.file_handle>> = Util.mk_ref None
+let get_qfile () = 
+    match !qfh with 
+        | Some f -> f
+        | None -> 
+          let fh = Util.open_file_for_writing "queries.smt2" in
+          qfh := Some fh;
+          fh
 
-let callZ3Exe (debug:bool) (theory:decls) labels = 
-  let theory = labels |> List.fold_left (fun decls (lname, t) -> decls@[Echo lname; Eval t]) theory in
-  let input = List.map declToSmt (theory@[Echo "Done!"]) |> String.concat "\n" in
-    if debug then Util.write_file (qfile()) input; 
+let cleanup () = 
+    Util.kill_process z3proc;
+    match !qfh with 
+        | Some f -> Util.close_file f
+        | _ -> ()
+
+let callZ3Exe (debug:bool) (theory:decls)  = 
+  let input = List.map declToSmt theory |> String.concat "\n" in
+    if debug then Util.append_to_file (get_qfile()) input;
     let status, lblnegs = doZ3Exe input in
     match status with 
-     | UNSAT -> true
-     | _ -> 
-       print_string <| format1 "Z3 says: %s\n" (status_to_string status);
-       match status with 
-         | UNKNOWN -> 
-           print_string <| format1 "Failing assertions: %s\n" (String.concat "\n\t" lblnegs); false
-         | _ -> 
-           print_string <| format1 "Failing assertions: %s\n" (String.concat "\n\t" lblnegs); false 
+        | UNSAT -> true
+        | _ -> 
+        print_string <| format1 "Z3 says: %s\n" (status_to_string status);
+        match status with 
+            | UNKNOWN -> 
+            print_string <| format1 "Failing assertions: %s\n" (String.concat "\n\t" lblnegs); false
+            | _ -> 
+            print_string <| format1 "Failing assertions: %s\n" (String.concat "\n\t" lblnegs); false 
