lib/system.fst
@@ -1,0 +1,11 @@
+module System
+assume type Object
+
+module System.IO
+assume type TextWriter
+
+module System.Text
+assume type StringBuilder
+
+module System.Diagnostics
+assume type Process
